Prepare registers for function calls

Definitions.thy
@@ -32,7 +32,6 @@ datatype llvm_compare_condition = comp_eq | comp_ne
                                 | comp_sgt | comp_sge | comp_slt | comp_sle
 type_synonym llvm_same_sign = bool
 
-
 datatype llvm_phi_node = phi llvm_identifier llvm_type "(llvm_identifier * llvm_value_ref) list"
 
 
@@ -41,6 +40,7 @@ datatype llvm_instruction = alloca llvm_identifier llvm_type "llvm_align option"
                           | load llvm_identifier llvm_type llvm_pointer "llvm_align option"
                           | add llvm_identifier llvm_add_wrap llvm_type llvm_value_ref llvm_value_ref
                           | icmp llvm_identifier llvm_same_sign llvm_compare_condition llvm_type llvm_value_ref llvm_value_ref
+                          | call llvm_type llvm_identifier "(llvm_type * llvm_value_ref) list"
 
 datatype llvm_terminator_instruction = ret llvm_type llvm_value_ref
                                      | br_i1 llvm_value_ref llvm_identifier llvm_identifier
@@ -56,16 +56,10 @@ type_synonym llvm_labeled_blocks = "(llvm_identifier * llvm_instruction_block) l
 datatype llvm_block_return = return_value llvm_value
                            | branch_label llvm_identifier
 
-datatype llvm_function_definition = func_def string llvm_type
-
-datatype llvm_function = func llvm_function_definition (blocks: llvm_labeled_blocks)
+datatype llvm_function = func llvm_type (blocks: llvm_labeled_blocks)
 hide_const (open) llvm_function.blocks
 
-datatype llvm_metadata = meta string string string
-
-type_synonym llvm_attributes = "string list"
-
-datatype llvm_program = program llvm_metadata "llvm_function list" llvm_attributes
+datatype llvm_program = program "(llvm_identifier * llvm_function) list"
 
 
 
@@ -75,7 +69,7 @@ section "Registers and Memory"
 subsection "Definitions"
 
 type_synonym ('n, 'v) register = "('n, 'v) mapping"
-type_synonym llvm_register_model = "(llvm_identifier, llvm_value) register"
+type_synonym llvm_register_model = "(string, llvm_value) register"
 
 definition empty_register :: "('n, 'v) register" where
   "empty_register = Mapping.empty"
@@ -88,56 +82,57 @@ type_synonym llvm_memory_model = "llvm_value memory_model"
 definition empty_memory :: "'a memory_model" where
   "empty_memory = []"
 
-type_synonym state = "llvm_register_model * llvm_memory_model * llvm_memory_model"
+
+type_synonym state = "llvm_register_model * llvm_register_model * llvm_memory_model * llvm_memory_model"
 
 definition empty_state :: "state" where
-  "empty_state = (empty_register, empty_memory, empty_memory)"
+  "empty_state = (empty_register, empty_register, empty_memory, empty_memory)"
 
 
 subsection "Register operations"
 
 (* Get *)
-
-fun get_register_value :: "('n, 'v) register \<Rightarrow> 'n \<Rightarrow> 'v result" where
-  "get_register_value vs n = (case Mapping.lookup vs n of None \<Rightarrow> err unknown_register_name | Some v \<Rightarrow> ok v)"
+fun get_single_register :: "('n, 'v) register \<Rightarrow> 'n \<Rightarrow> 'v result" where
+  "get_single_register r n = (case Mapping.lookup r n of None \<Rightarrow> err unknown_register_name | Some v \<Rightarrow> ok v)"
 
 fun get_register :: "state \<Rightarrow> llvm_value_ref \<Rightarrow> llvm_value result" where
   "get_register _ (val v) = ok v"
-| "get_register (vs,s,h) (reg n) = get_register_value vs n"
+| "get_register (l,g,s,h) (reg (lid n)) = get_single_register l n"
+| "get_register (l,g,s,h) (reg (gid n)) = get_single_register g n"
+
 
 (* Set *)
-
-definition set_register_value :: "'n \<Rightarrow> 'v \<Rightarrow> ('n, 'v) register \<Rightarrow> ('n, 'v) register" where
-  "set_register_value n v vs = Mapping.update n v vs"
+definition set_single_register :: "'n \<Rightarrow> 'v \<Rightarrow> ('n, 'v) register \<Rightarrow> ('n, 'v) register" where
+  "set_single_register n v r = Mapping.update n v r"
 
 fun set_register :: "llvm_identifier \<Rightarrow> llvm_value \<Rightarrow> state \<Rightarrow> state" where
-  "set_register n v (vs,s,h) = (set_register_value n v vs,s,h)"
+  "set_register (lid n) v (l,g,s,h) = (set_single_register n v l,g,s,h)"
+| "set_register (gid n) v (l,g,s,h) = (l,set_single_register n v g,s,h)"
 
 
 subsection "Memory operations"
 
 (* Allocate *)
-
 definition allocate_single_memory :: "'a memory_model \<Rightarrow> ('a memory_model * memory_model_address)" where
   "allocate_single_memory m = (m@[mem_unset], length m)"
 
 definition allocate_stack :: "state \<Rightarrow> (state * llvm_address)" where
-  "allocate_stack s = (case s of (vs,s,h) \<Rightarrow> let (s', a) = allocate_single_memory s in ((vs,s',h), saddr a))"
+  "allocate_stack s = (case s of (l,g,s,h) \<Rightarrow> let (s', a) = allocate_single_memory s in ((l,g,s',h), saddr a))"
 
 definition allocate_heap :: "state \<Rightarrow> (state * llvm_address)" where
-  "allocate_heap s = (case s of (vs,s,h) \<Rightarrow> let (h', a) = allocate_single_memory h in ((vs,s,h'), haddr a))"
+  "allocate_heap s = (case s of (l,g,s,h) \<Rightarrow> let (h', a) = allocate_single_memory h in ((l,g,s,h'), haddr a))"
+
 
 (* Address validity *)
-
 definition valid_single_memory_address :: "'a memory_model \<Rightarrow> memory_model_address \<Rightarrow> bool" where
   "valid_single_memory_address m a = (a < length m \<and> m!a \<noteq> mem_freed)"
 
 fun valid_memory_address :: "state \<Rightarrow> llvm_address \<Rightarrow> bool" where
-  "valid_memory_address (vs,s,h) (haddr a) = valid_single_memory_address h a"
-| "valid_memory_address (vs,s,h) (saddr a) = valid_single_memory_address s a"
+  "valid_memory_address (l,g,s,h) (haddr a) = valid_single_memory_address h a"
+| "valid_memory_address (l,g,s,h) (saddr a) = valid_single_memory_address s a"
+
 
 (* Get *)
-
 definition get_single_memory :: "'a memory_model \<Rightarrow> memory_model_address \<Rightarrow> 'a result" where
   "get_single_memory m a = do {
     assert unallocated_address (valid_single_memory_address m a);
@@ -148,11 +143,11 @@ definition get_single_memory :: "'a memory_model \<Rightarrow> memory_model_addr
   }"
 
 fun get_memory :: "state \<Rightarrow> llvm_address \<Rightarrow> llvm_value result" where
-  "get_memory (vs,s,h) (haddr a) = get_single_memory h a"
-| "get_memory (vs,s,h) (saddr a) = get_single_memory s a"
+  "get_memory (l,g,s,h) (haddr a) = get_single_memory h a"
+| "get_memory (l,g,s,h) (saddr a) = get_single_memory s a"
+
 
 (* Set *)
-
 definition set_single_memory :: "memory_model_address \<Rightarrow> 'a \<Rightarrow> 'a memory_model \<Rightarrow> 'a memory_model result" where
   "set_single_memory a v m = do {
     assert unallocated_address (valid_single_memory_address m a);
@@ -160,17 +155,17 @@ definition set_single_memory :: "memory_model_address \<Rightarrow> 'a \<Rightar
   }"
 
 fun set_memory :: "llvm_address \<Rightarrow> llvm_value \<Rightarrow> state \<Rightarrow> state result" where
-  "set_memory (haddr a) v (r,s,h) = do {
+  "set_memory (haddr a) v (l,g,s,h) = do {
     h' \<leftarrow> set_single_memory a v h;
-    return (r,s,h')
+    return (l,g,s,h')
   }"
-| "set_memory (saddr a) v (r,s,h) = do {
+| "set_memory (saddr a) v (l,g,s,h) = do {
     s' \<leftarrow> set_single_memory a v s;
-    return (r,s',h)
+    return (l,g,s',h)
   }"
+
 
 (* Free *)
-
 definition free_single_memory :: "memory_model_address \<Rightarrow> 'a memory_model \<Rightarrow> 'a memory_model result" where
   "free_single_memory a m = do {
     assert unallocated_address (valid_single_memory_address m a);
@@ -178,13 +173,13 @@ definition free_single_memory :: "memory_model_address \<Rightarrow> 'a memory_m
   }"
 
 fun free_memory :: "llvm_address \<Rightarrow> state \<Rightarrow> state result" where
-  "free_memory (haddr a) (r,s,h) = do {
+  "free_memory (haddr a) (l,g,s,h) = do {
     h' \<leftarrow> free_single_memory a h;
-    return (r,s,h')
+    return (l,g,s,h')
   }"
-| "free_memory (saddr a) (r,s,h) = do {
+| "free_memory (saddr a) (l,g,s,h) = do {
     s' \<leftarrow> free_single_memory a s;
-    return (r,s',h)
+    return (l,g,s',h)
   }"
 
 
@@ -202,14 +197,15 @@ definition single_memory_\<alpha> where
   else None"
 
 fun memory_\<alpha> :: "state \<Rightarrow> llvm_address \<Rightarrow> llvm_value option option" where
-  "memory_\<alpha> (vs,s,h) (saddr a) = single_memory_\<alpha> s a"
-| "memory_\<alpha> (vs,s,h) (haddr a) = single_memory_\<alpha> h a"
+  "memory_\<alpha> (l,g,s,h) (saddr a) = single_memory_\<alpha> s a"
+| "memory_\<alpha> (l,g,s,h) (haddr a) = single_memory_\<alpha> h a"
 
 
 subsection "Register"
 
 fun register_\<alpha> :: "state \<Rightarrow> llvm_value_ref \<Rightarrow> llvm_value option" where
-  "register_\<alpha> (vs,s,h) (val v) = Some v"
-| "register_\<alpha> (vs,s,h) (reg n) = Mapping.lookup vs n"
+  "register_\<alpha> (l,g,s,h) (val v) = Some v"
+| "register_\<alpha> (l,g,s,h) (reg (lid n)) = Mapping.lookup l n"
+| "register_\<alpha> (l,g,s,h) (reg (gid n)) = Mapping.lookup g n"
 
 end
