Registers.thy
@@ -4,16 +4,24 @@ begin
 
 section "Simps"
 
-lemma memory_\<alpha>_eq[simp]: "memory_\<alpha> (r,s,h) = memory_\<alpha> (r',s,h)"
+lemma memory_\<alpha>_eq[simp]: "memory_\<alpha> (l,g,s,h) = memory_\<alpha> (l',g',s,h)"
   apply (rule ext)
   subgoal for x
     by (cases x; simp)
   done
 
-lemma register_\<alpha>_update_eq[simp]:
-  "register_\<alpha> (Mapping.update n v r, s, h) = (register_\<alpha> (r, s, h))(reg n := Some v)"
+lemma register_\<alpha>_lid_update_eq[simp]:
+  "register_\<alpha> (Mapping.update n v l, g, s, h) = (register_\<alpha> (l, g, s, h))(reg (lid n) := Some v)"
   apply (auto simp: fun_eq_iff split: llvm_value_ref.split)
-  subgoal for x by (cases x; simp)
+  subgoal for x apply (cases x; simp) subgoal for id by (cases id; simp)
+  done
+  done
+
+lemma register_\<alpha>_gid_update_eq[simp]:
+  "register_\<alpha> (l, Mapping.update n v g, s, h) = (register_\<alpha> (l, g, s, h))(reg (gid n) := Some v)"
+  apply (auto simp: fun_eq_iff split: llvm_value_ref.split)
+  subgoal for x apply (cases x; simp) subgoal for id by (cases id; simp)
+  done
   done
 
 lemma register_\<alpha>_val_eq[simp]:
@@ -31,7 +39,7 @@ section "register_\<alpha> operation"
 lemma set_register_\<alpha>:
   "register_\<alpha> (set_register n v s) = (register_\<alpha> s)(reg n := Some v)"
   apply (cases s; rule ext)
-  subgoal for r' s' h' x by (cases x; auto simp: set_register_value_def)
+  subgoal for l' g' s' h' x by (cases x; cases n; auto simp: set_single_register_def)
   done
 
 
@@ -40,20 +48,26 @@ section "Intro rules"
 
 named_theorems register_intro
 
-lemma wp_set_register_value_intro[THEN consequence, register_intro]:
-  "wp (return (set_register_value n v r,s,h)) (\<lambda>s'. register_\<alpha> s' = (register_\<alpha> (r,s,h))(reg n := Some v) \<and> memory_\<alpha> s' = memory_\<alpha> (vs,s,h))"
-  unfolding set_register_value_def
+lemma wp_set_single_register_lid_intro[THEN consequence, register_intro]:
+  "wp (return (set_single_register n v l,g,s,h)) (\<lambda>s'. register_\<alpha> s' = (register_\<alpha> (l,g,s,h))(reg (lid n) := Some v) \<and> memory_\<alpha> s' = memory_\<alpha> (l,g,s,h))"
+  unfolding set_single_register_def
+  by (intro wp_intro wp_return_intro; simp)
+
+lemma wp_set_single_register_gid_intro[THEN consequence, register_intro]:
+  "wp (return (l,set_single_register n v g,s,h)) (\<lambda>s'. register_\<alpha> s' = (register_\<alpha> (l,g,s,h))(reg (gid n) := Some v) \<and> memory_\<alpha> s' = memory_\<alpha> (l,g,s,h))"
+  unfolding set_single_register_def
   by (intro wp_intro wp_return_intro; simp)
 
 lemma wp_set_register_intro[THEN consequence, wp_intro]:
   shows "wp (return (set_register n v s)) (\<lambda>s'. register_\<alpha> s' = (register_\<alpha> s)(reg n := Some v) \<and> memory_\<alpha> s' = memory_\<alpha> s)"
-  by (cases s; simp; intro wp_intro register_intro; simp)
+  by (cases n; cases s; simp; intro wp_intro register_intro; simp)
 
 
 lemma wp_get_register_intro[THEN consequence, wp_intro]:        
   assumes "register_\<alpha> s n \<noteq> None"
   shows "wp (get_register s n) (\<lambda>v'. register_\<alpha> s n = Some v')"
   using assms
-  by (cases s; cases n; simp; intro wp_intro; auto)
+  apply (cases s; cases n) subgoal for _ _ _ _ id by (cases id; simp; intro wp_intro; auto)
+  by simp
 
 end
